\section{Brownian Motion}

假设连续随机过程$X_t$满足

\begin{equation}
    \ud X_t = a(X,t)\ud t + b(X,t)\ud z
\end{equation}

随机微分方程的与一般微分方程的区别核心是

\begin{equation}\label{eq_z2t}
    (\ud z)^2 = \ud t
\end{equation}

由\ref{eq_z2t}知道

\begin{equation}
    (\ud X_t)^2 = b^2(X_t,t) (\ud z)^2 = b^2(X_t,t) \ud t
\end{equation}

由Ito公式，对$G(X_t)$

\begin{equation}\label{eq_ud_G}
    \begin{array}{rcl}
        \ud G(X_t,t) & = & \frac{\partial G}{\partial X_t}\ud X_t + \frac{\partial G}{\partial t}\ud t + \frac{1}{2}\frac{\partial^2 G}{\partial X_t^2} (\ud X_t)^2      \\
                     & = & \frac{\partial G}{\partial X_t}\ud X_t + \frac{\partial G}{\partial t}\ud t + \frac{1}{2}\frac{\partial^2 G}{\partial X_t^2} b^2(X_t,t) \ud t
    \end{array}
\end{equation}

取$G(X_t,t) = \ln X_t, a(X_t,t) = \mu X_t, b(X_t,t) = \sigma X_t$，则

\begin{equation}
    \frac{\ud X_t}{X_t} = \mu \ud t + \sigma \ud z
\end{equation}

以及

\begin{equation}
    \frac{\partial G}{\partial X_t} = \frac{1}{X_t},\quad \frac{\partial G}{\partial t} = 0, \quad \frac{\partial^2 G}{\partial X_t^2} = -\frac{1}{X_t^2}
\end{equation}

将这些结果带入\ref{eq_ud_G}中有

\begin{equation}
    \begin{array}{rcl}
        \ud \ln X_t & = & \frac{\ud X_t}{X_t} + 0\cdot\ud t -\frac{1}{2}\frac{1}{X_t^2}X_t^2\sigma^2\ud t \\
                    & = & \mu\ud t + \sigma \ud z - \frac{\sigma^2}{2}\ud t                               \\
                    & = & (\mu - \frac{\sigma^2}{2})\ud t + \sigma \ud z
    \end{array}
\end{equation}

由此可知

\begin{equation}
    \ln X_T - \ln X_0 \sim \N((\mu - \frac{\sigma^2}{2})T, \sigma^2T)
\end{equation}

或者

\begin{equation}
    \ln X_T  \sim \N(\ln X_0 + (\mu - \frac{\sigma^2}{2})T, \sigma^2T) = \N(\mu', \sigma'^2)
\end{equation}

其中

\begin{equation}
    \mu' = \ln X_0 + (\mu - \frac{\sigma^2}{2})T, \sigma'^2 = \sigma^2T
\end{equation}

使用公式\ref{eq_lognorm_e1}可知

\begin{equation}
    \E X_T = e^{\mu' + \frac{\sigma'^2}{2}} = e^{\ln X_0 + \mu T} = X_0e^{\mu T}
\end{equation}

综上即有

\begin{equation}
    \left\{
    \begin{array}{rcl}
        \ln \E \frac{X_T}{X_0} & = & \mu T                       \\
        \E \ln \frac{X_T}{X_0} & = & \mu T - \frac{\sigma^2T}{2}
    \end{array}
    \right.
\end{equation}

参考附录中的代码 \ref{sub_sec_code_block_bm_pah}