\section{Log Norm}

\subsection{定义}

已知非负随机变量$X$满足参数为$(\mu,\sigma)$对数正态分布，即

\begin{equation}
    \ln{X} \sim \rm{N}(\mu,\sigma^2)
\end{equation}

\subsection{分布函数}

\begin{equation}
    \begin{array}{rcl}
        F(x) & = & \Pr(X \leq x)                     \\
             & = & \Pr(\ln X \leq \ln x)             \\
             & = & \Phi (\frac{\ln x - \mu}{\sigma})
    \end{array}
\end{equation}

\subsection{概率密度}

\begin{equation}\label{eq_lognorm_prob_density}
    \begin{array}{rcl}
        f(x) & = & F'(x)                                                                                   \\
             & = & \Phi' (\frac{\ln x - \mu}{\sigma}) (\frac{\ln x - \mu}{\sigma})'                        \\
             & = & \frac{1}{\sqrt{2\pi\sigma^2}}\exp\{-\frac{(\ln x - \mu)^2}{2\sigma^2}\}\cdot\frac{1}{x}
    \end{array}
\end{equation}

\subsection{期望}

记$z = \frac{\ln x - \mu}{\sigma}$，则$x = \exp\{\sigma z + \mu\}$， 从而

\begin{equation}
    \ud x = \exp(\sigma z + \mu)\sigma \ud z
\end{equation}

于是

\begin{equation}\label{eq_lognorm_e1}
    \begin{array}{rcl}
        \E X & = & \int_0^\infty xf(x)\ud x                                                                                                        \\
             & = & \int_0^\infty \frac{1}{\sqrt{2\pi\sigma^2}}\exp\{-\frac{(\ln x - \mu)^2}{2\sigma^2}\}\ud x                                      \\
             & = & \int_{-\infty}^\infty\frac{1}{\sqrt{2\pi}}\exp\{-\frac{z^2}{2}\} \exp\{\sigma z + \mu\} \ud z                                     \\
             & = & \int_{-\infty}^\infty\frac{1}{\sqrt{2\pi}}\exp\{-\frac{z^2}{2}+ \sigma z -\frac{\sigma^2}{2} + \mu + \frac{\sigma^2}{2}\} \ud z \\
             & = & \exp\{\mu + \frac{\sigma^2}{2}\}\int_{-\infty}^\infty\frac{1}{\sqrt{2\pi}}\exp\{ -\frac{(z-\sigma)^2}{2}\} \ud z                  \\
             & = & \exp\{\mu + \frac{\sigma^2}{2}\}
    \end{array}
\end{equation}

\subsection{方差}
\begin{equation}
    \begin{array}{rcl}
        \E X^2 & = & \int_0^\infty x^2f(x)\ud x                                                                                                        \\
               & = & \int_0^\infty \frac{1}{\sqrt{2\pi\sigma^2}}\exp\{-\frac{(\ln x - \mu)^2}{2\sigma^2}\}x\ud x                                      \\
               & = & \int_{-\infty}^\infty\frac{1}{\sqrt{2\pi}}\exp\{-\frac{z^2}{2}\} \exp\{2\sigma z + 2\mu\} \ud z                                     \\
               & = & \int_{-\infty}^\infty\frac{1}{\sqrt{2\pi}}\exp\{-\frac{z^2}{2}+ 2\sigma z -2\sigma^2 + 2\mu + 2\sigma^2\} \ud z \\
               & = & \exp\{2\mu + 2\sigma^2\}\int_{-\infty}^\infty\frac{1}{\sqrt{2\pi}}\exp\{ -\frac{(z-2\sigma)^2}{2}\} \ud z                  \\
               & = & \exp\{2\mu + 2\sigma^2\}
    \end{array}
\end{equation}

从而

\begin{equation}
    \Var(X) = \E X^2 - (\E X )^2 = e^{2\mu+\sigma^2}(e^{\sigma^2}-1)
\end{equation}

\subsection{小结}

一方面，由于$\ln(\cdot)$的凹函数性质，可知

\begin{equation}
    \E \ln(X) \leq \ln(\E X)
\end{equation}

另一方面，经过计算，可以直接验证该结论。

\begin{equation}
    \mu = \E \ln(X) \leq \ln(\E X) = \mu + \frac{\sigma^2}{2}
\end{equation}